Add final Properties file for symmetry's sake, add defs and thms into Property files that didn't have them yet

project/Bounded_Elementary_CA.thy
@@ -22,38 +22,4 @@ fun update_CA :: "CA \<Rightarrow> CA" where
 
 fun run_t_steps :: "CA \<Rightarrow> nat \<Rightarrow> CA" where
 "run_t_steps ca n = apply_t_times update_CA ca n"
-
-definition yields :: "CA \<Rightarrow> state \<Rightarrow> bool" (infixr \<open>yields\<close>  65) where
-"A yields s \<equiv> (\<exists> n. State (run_t_steps A n) = s \<and> n > 0)"
-
-definition loops :: "CA \<Rightarrow> bool" where
-"loops ca \<equiv> ca yields State ca"
-
-(* maybe add some infix notation for this *)
-(* maybe change to run_t_steps 1 for more precision *)
-fun garden_of_eden :: "CA \<Rightarrow> bool" where
-"garden_of_eden (CA s r) = (\<not>(\<exists> s0. (CA s0 r) yields s))"
-
-fun reversible :: "CA \<Rightarrow> bool" where
-"reversible (CA _ r) = (\<forall>s. (\<exists>!s0. State (update_CA (CA s0 r)) = s))"
-
-theorem "ca yields State (run_t_steps ca 1)"
-proof-
-  show ?thesis using yields_def by blast
-qed
-
-theorem t1 :"n>0 \<Longrightarrow> ca yields State (run_t_steps ca n)"
-  apply(simp add: yields_def)
-  apply(rule exI)
-  apply(rule conjI)
-  apply(auto)
-  done
-
-
-theorem "testCA yields [Zero, Zero, Zero]"
-  apply(simp add: yields_def)
-  apply(rule_tac x=1 in exI)
-  apply(rule conjI)
-   apply(auto)
-  sorry
 end
