project/Bounded_Elementary_CA_Properties.thy
@@ -1,11 +1,6 @@
-theory Toroidal_Elementary_CA_Properties
-  imports Toroidal_Elementary_CA
+theory Bounded_Elementary_CA_Properties
+  imports Bounded_Elementary_CA
 begin
-
-section \<open>Important Property Definitions\<close>
-
-definition stable :: "CA \<Rightarrow> bool" where
-"stable ca \<equiv> State (update_CA ca) = State ca"
 
 definition yields :: "CA \<Rightarrow> state \<Rightarrow> bool" (infixr \<open>yields\<close>  65) where
 "A yields s \<equiv> (\<exists> n. State (run_t_steps A n) = s \<and> n > 0)"
@@ -13,7 +8,11 @@ definition yields :: "CA \<Rightarrow> state \<Rightarrow> bool" (infixr \<open>
 definition loops :: "CA \<Rightarrow> bool" where
 "loops ca \<equiv> ca yields State ca"
 
-(* TODO reframe in terms of rules only *)
+(* maybe add some infix notation for this *)
+(* maybe change to run_t_steps 1 for more precision *)
+fun garden_of_eden :: "CA \<Rightarrow> bool" where
+"garden_of_eden (CA s r) = (\<not>(\<exists> s0. (CA s0 r) yields s))"
+
 fun reversible :: "CA \<Rightarrow> bool" where
 "reversible (CA _ r) = (\<forall>s. (\<exists>!s0. State (update_CA (CA s0 r)) = s))"
 
@@ -30,18 +29,10 @@ theorem t1 :"n>0 \<Longrightarrow> ca yields State (run_t_steps ca n)"
   done
 
 
-(* maybe add some infix notation for this or other things as it looks good *)
-fun garden_of_eden :: "CA \<Rightarrow> bool" where
-"garden_of_eden (CA s r) = (\<not>(\<exists> s0. State (update_CA (CA s0 r)) = s))"
-
 definition orphan :: "state \<Rightarrow> rule \<Rightarrow> bool" where
 "orphan s0 r = (\<forall> sl sr. garden_of_eden (CA (sl@s0@sr) r))"
 
 lemma "garden_of_eden ca \<Longrightarrow> \<not>reversible ca"
-  apply (metis garden_of_eden.elims(2) reversible.simps)
-done
-
-(*lemma "garden_of_eden (CA s r) \<Longrightarrow> (\<exists> s0. (orphan s0 r) \<and> (\<exists> sl sr. (sl@s0@sr) = s))"*)
 
 definition class1 :: "rule \<Rightarrow> bool" where
 "class1 r \<equiv> (\<exists>! f. (\<forall> s. (CA s r) yields f \<and> uniform f \<and> stable (CA f r)))"
