project/Toroidal_TwoDim_CA_Properties.thy
@@ -1,11 +1,12 @@
-theory Toroidal_Elementary_CA_Properties
-  imports Toroidal_Elementary_CA
+theory Toroidal_TwoDim_CA_Properties
+  imports Toroidal_TwoDim_CA
 begin
-
-section \<open>Important Property Definitions\<close>
 
 definition stable :: "CA \<Rightarrow> bool" where
 "stable ca \<equiv> State (update_CA ca) = State ca"
+
+definition uniform :: "state \<Rightarrow> bool" where
+"uniform s \<equiv> length (remdups (concat s)) = 1"
 
 definition yields :: "CA \<Rightarrow> state \<Rightarrow> bool" (infixr \<open>yields\<close>  65) where
 "A yields s \<equiv> (\<exists> n. State (run_t_steps A n) = s \<and> n > 0)"
@@ -13,35 +14,15 @@ definition yields :: "CA \<Rightarrow> state \<Rightarrow> bool" (infixr \<open>
 definition loops :: "CA \<Rightarrow> bool" where
 "loops ca \<equiv> ca yields State ca"
 
-(* TODO reframe in terms of rules only *)
 fun reversible :: "CA \<Rightarrow> bool" where
 "reversible (CA _ r) = (\<forall>s. (\<exists>!s0. State (update_CA (CA s0 r)) = s))"
 
-theorem "ca yields State (run_t_steps ca 1)"
-proof-
-  show ?thesis using yields_def by blast
-qed
-
-theorem t1 :"n>0 \<Longrightarrow> ca yields State (run_t_steps ca n)"
-  apply(simp add: yields_def)
-  apply(rule exI)
-  apply(rule conjI)
-  apply(auto)
-  done
-
-
-(* maybe add some infix notation for this or other things as it looks good *)
 fun garden_of_eden :: "CA \<Rightarrow> bool" where
 "garden_of_eden (CA s r) = (\<not>(\<exists> s0. State (update_CA (CA s0 r)) = s))"
 
-definition orphan :: "state \<Rightarrow> rule \<Rightarrow> bool" where
-"orphan s0 r = (\<forall> sl sr. garden_of_eden (CA (sl@s0@sr) r))"
-
 lemma "garden_of_eden ca \<Longrightarrow> \<not>reversible ca"
-  apply (metis garden_of_eden.elims(2) reversible.simps)
-done
+  by (metis garden_of_eden.elims(2) reversible.simps)
 
-(*lemma "garden_of_eden (CA s r) \<Longrightarrow> (\<exists> s0. (orphan s0 r) \<and> (\<exists> sl sr. (sl@s0@sr) = s))"*)
 
 definition class1 :: "rule \<Rightarrow> bool" where
 "class1 r \<equiv> (\<exists>! f. (\<forall> s. (CA s r) yields f \<and> uniform f \<and> stable (CA f r)))"
